Remove R from lock spec

atomic/lock.v
@@ -18,38 +18,38 @@ Section proof.
   Definition acquired (lk: val) : iProp Σ :=
     ∃ (l: loc), ⌜ lk = #l ⌝ ∗ l ↦{#3 / 4} #true.
 
-  Definition lock (lk: val) (st: state) (R: iProp Σ) : iProp Σ := 
+  Definition lock (lk: val) (st: state) : iProp Σ := 
     ∃ (l: loc), ⌜ lk = #l ⌝ ∗ 
     match st with
-    | Free => l ↦ #false ∗ R
+    | Free => l ↦ #false
     | Locked => l ↦{#1 / 4} #true
     end.
 
-  Global Instance lock_timeless lk st R `{!Timeless R} : Timeless (lock lk st R).
+  Global Instance lock_timeless lk st : Timeless (lock lk st).
   Proof. destruct st; apply _. Qed.
 
-  Lemma newlock_spec (R : iProp Σ) :
-    {{{ R }}} newlock #() {{{ lk, RET lk; lock lk Free R }}}.
+  Lemma newlock_spec :
+    {{{ emp }}} newlock #() {{{ lk, RET lk; lock lk Free }}}.
   Proof.
-    iIntros (Φ) "HR HΦ". wp_lam. wp_alloc l as "Hl".
+    iIntros (Φ) "_ HΦ". wp_lam. wp_alloc l as "Hl".
     iModIntro; iApply "HΦ". iExists l. by iFrame.
   Qed.
 
-  Lemma try_acquire_spec (lk: val) (R : iProp Σ) :
-    ⊢ <<< ∀∀ st, lock lk st R >>> try_acquire lk @ ∅
-    <<< ∃∃ b, lock lk Locked R ∗ ⌜ if b is true then st = Free else st = Locked ⌝, RET #b >>>
-    {{{ if b is true then acquired lk ∗ R else emp }}}.
+  Lemma try_acquire_spec (lk: val) :
+    ⊢ <<< ∀∀ st, lock lk st >>> try_acquire lk @ ∅
+    <<< ∃∃ b, lock lk Locked ∗ ⌜ if b is true then st = Free else st = Locked ⌝, RET #b >>>
+    {{{ if b is true then acquired lk else emp }}}.
   Proof.
     iIntros (Φ) "AU"; rewrite difference_empty_L.
     wp_lam. wp_bind (CmpXchg _ _ _).
     iMod "AU" as ([]) "[Hlock [_ Hclose]]".
-    + iDestruct "Hlock" as (l) "[-> [Hl HR]]". wp_cmpxchg_suc.
+    + iDestruct "Hlock" as (l) "[-> Hl]". wp_cmpxchg_suc.
       rewrite -Qp.quarter_three_quarter; iDestruct "Hl" as "(Hl & Hl')".
       iDestruct ("Hclose" $! true with "[Hl]") as ">AP".
       { iSplit; last done. iExists l. by iFrame. }
       iMod (atomic_post_commit with "AP") as "HΦ".
-      iModIntro; wp_pures. iApply "HΦ". 
-      iFrame "HR". iExists l. by iFrame.
+      iModIntro; wp_pures. iApply "HΦ".
+      iExists l. by iFrame.
     + iDestruct "Hlock" as (l) "[-> Hl]". wp_cmpxchg_fail.
       iDestruct ("Hclose" $! false with "[Hl]") as ">AP".
       { iSplit; last done. iExists l. by iFrame. }
@@ -57,10 +57,10 @@ Section proof.
       iModIntro; wp_pures. by iApply "HΦ".
   Qed.
 
-  Lemma acquire_spec (lk: val) (R : iProp Σ) :
-    ⊢ <<< ∀∀ st, lock lk st R >>> acquire lk @ ∅ 
-    <<< lock lk Locked R ∗ ⌜ st = Free ⌝, RET #() >>>
-    {{{ acquired lk ∗ R }}}.
+  Lemma acquire_spec (lk: val) :
+    ⊢ <<< ∀∀ st, lock lk st >>> acquire lk @ ∅ 
+    <<< lock lk Locked ∗ ⌜ st = Free ⌝, RET #() >>>
+    {{{ acquired lk }}}.
   Proof.
     iIntros (Φ) "AU"; rewrite difference_empty_L.
     iLöb as "IH". wp_lam.
@@ -69,28 +69,28 @@ Section proof.
     iIntros (st) "Hlock"; iAaccIntro with "Hlock".
     { do 2 (iIntros; iModIntro; iFrame). }
     iIntros ([]) "[Hlock ->]".
-    + iModIntro. iExists Locked. iFrame "Hlock". iIntros "Hlock". 
+    + iModIntro. iExists Locked. iFrame "Hlock". iIntros "Hlock".
       iRight. iFrame. iSplit; first done. iIntros "AP".
       iMod (atomic_post_commit with "AP") as "HΦ".
       by iModIntro; iIntros; iModIntro; wp_pures; iApply "HΦ".
-    + iModIntro. iExists Locked. iFrame "Hlock". iIntros "Hlock". 
-      iLeft. iFrame. iIntros "AP". 
+    + iModIntro. iExists Locked. iFrame "Hlock". iIntros "Hlock".
+      iLeft. iFrame. iIntros "AP".
       by iModIntro; iIntros; iModIntro; wp_pures; iApply "IH".
   Qed.
 
-  Lemma release_spec (lk: val) (R : iProp Σ) :
-    acquired lk -∗ R -∗
-    <<< ∀∀ st, lock lk st R >>> release lk @ ∅
-    <<< lock lk Free R, RET #() >>>
+  Lemma release_spec (lk: val) :
+    acquired lk -∗
+    <<< ∀∀ st, lock lk st >>> release lk @ ∅
+    <<< lock lk Free, RET #() >>>
     {{{ emp }}}.
   Proof.
-    iIntros "Hacq HR" (Φ) "AU"; rewrite difference_empty_L.
+    iIntros "Hacq" (Φ) "AU"; rewrite difference_empty_L.
     iDestruct "Hacq" as (l) "[-> Hl]".
     wp_lam. iMod "AU" as ([]) "[Hlock [_ Hclose]]";
-      iDestruct "Hlock" as (l') "[%Heq [Hl' HR']]"; replace l' with l by congruence.
+      iDestruct "Hlock" as (l') "[%Heq Hl']"; replace l' with l by congruence.
     { iDestruct (mapsto_agree with "Hl Hl'") as %?; congruence. }
-    iCombine "Hl Hl' HR'" as "Hl"; rewrite Qp.three_quarter_quarter.
-    wp_store. iMod ("Hclose" with "[Hl HR]") as "AP".
+    iCombine "Hl Hl'" as "Hl"; rewrite Qp.three_quarter_quarter.
+    wp_store. iMod ("Hclose" with "[Hl]") as "AP".
     { iExists l. by iFrame. }
     iMod "AP" as (st) "[Hlock [_ HΦ]]". 
     iMod ("HΦ" with "Hlock") as "HΦ".
